add while rule

hoare.bpl
@@ -3,11 +3,15 @@ type Val;
 type Expr;
 type State;
 
+data Nat
+  = zero | succ(pred: Nat);
+
 data Cmd
   = skip
   | assign(lhs: Var, rhs: Expr)
   | seq(fst: Cmd, snd: Cmd)
   | if(test: Expr, left: Cmd, right: Cmd)
+  | while(cond: Expr, body: Cmd)
   ;
 
 function eval(expr: Expr, st: State): Val;
@@ -18,6 +22,7 @@ function update(st: State, lhs: Var, rhs: Val): State;
 function subst(prop: [State]bool, lhs: Var, rhs: Expr): [State]bool;
 
 function steps(cmd: Cmd, st: State, st_: State): bool;
+function iter(n: Nat, test: Expr, cmd: Cmd, st: State, st_: State): bool;
 
 axiom forall expr: Expr, st: State ::
   prop(expr)[st] == truth(eval(expr, st));
@@ -46,10 +51,22 @@ axiom forall fst: Cmd, snd: Cmd, st: State, st__: State ::
   steps(seq(fst, snd), st, st__)
     == (exists st_: State :: steps(fst, st, st_) && steps(snd, st_, st__));
 
+axiom forall test: Expr, body: Cmd, st: State, st_: State ::
+  iter(zero, test, body, st, st_)
+    == (!truth(eval(test, st)) && st_ == st);
+
+axiom forall n: Nat, test: Expr, body: Cmd, st: State, st__: State ::
+  iter(succ(n), test, body, st, st__)
+    == (truth(eval(test, st)) && exists st_: State :: steps(body, st, st_) && iter(n, test, body, st_, st__));
+
 axiom forall test: Expr, left: Cmd, right: Cmd, st: State, st_: State ::
   steps(if(test, left, right), st, st_)
     == (    truth(eval(test, st)) && steps(left,  st, st_)
         || !truth(eval(test, st)) && steps(right, st, st_));
+
+axiom forall test: Expr, body: Cmd, st: State, st_: State ::
+  steps(while(test, body), st, st_)
+    == exists n: Nat :: iter(n, test, body, st, st_);
 
 function hoare(pre: [State]bool, cmd: Cmd, post: [State]bool): bool {
   forall st: State, st_: State ::
@@ -71,3 +88,18 @@ lemma forall test: Expr, left: Cmd, right: Cmd, P: [State]bool, Q: [State]bool :
   hoare(and_(P, prop(test)), left, Q) &&
   hoare(and_(P, not_(prop(test))), right, Q)
     ==> hoare(P, if(test, left, right), Q);
+
+lemma forall n: Nat, test: Expr, body: Cmd, st: State, st_: State ::
+  iter(n, test, body, st, st_)
+    ==> ! truth(eval(test, st_))
+proof induction n end;
+
+lemma forall n: Nat, test: Expr, body: Cmd, I: [State]bool, st: State, st_: State ::
+  hoare(and_(I, prop(test)), body, I) &&
+  iter(n, test, body, st, st_) && I[st]
+    ==> I[st_]
+proof induction n end;
+
+lemma forall test: Expr, body: Cmd, I: [State]bool ::
+  hoare(and_(I, prop(test)), body, I)
+    ==> hoare(I, while(test, body), and_(I, not_(prop(test))));
